SignedDH: a start on the EasyCrypt proof

signedDH/easycrypt/SignedDH.ec
@@ -1,5 +1,8 @@
-require import AllCore FMap FSet Distr.
+require import AllCore Real FMap FSet Distr.
 require import PROM.
+
+require (*--*) StdOrder.
+(*---*) import StdOrder.RealOrder.
 
 require (*--*) St_CDH_abstract SUFCMA UATPaKE.
 
@@ -7,50 +10,35 @@ require (*--*) St_CDH_abstract SUFCMA UATPaKE.
 (* Starting notes:
    - We (try to) follow Doreen and Paul's model as closely as possible
      while remaining precise.
-   - Whenever the pen and paper definition takes adversarial input in
-     the form of a public key, that is then used to look for the
-     identity of the intended partner, we instead takes input as
-     "either a handle or a public key". This makes our definition more
-     precise (because we don't make an arbitrary choice when two
-     honest parties generate the same key), but also slightly more
-     complex.
-     In order to align with Doreen and Paul's model, we prevent the
-     adversary from presenting us with a public-key that is already
-     associated with a registered server. (Their definition infers
-     intent; we prefer to enforce that adversary actions match
-     intent.)
-   - We probably want signing to be expressed as a multi-forgery game.
-     (TODO: figure this out.)
    - The NIKE is split out as Nominal Group with Gap-DH + RO. The
      entire scheme could be proved assuming an abstract NIKE (with
      m-CKS-heavy security), and that be constructed from NG + Gap-DH +
      RO.
 *)
 
-(** Handles to refer to servers and client instances **)
-type s_handle, c_handle.
-
 (** Types and operators for the DH group **)
 type pdh, sdh, sskey.
 
-op [lossless] dkp: (pdh * sdh) distr.
-op shared_key: pdh -> sdh -> pdh.
+op g: pdh.
+op [lossless] dsk: sdh distr.
+op (^): pdh -> sdh -> pdh.
 
-axiom shared_keyC X x Y y:
-     (X, x) \in dkp
-  => (Y, y) \in dkp
-  => shared_key X y = shared_key Y x.
+axiom shared_keyC x y:
+     x \in dsk
+  => y \in dsk
+  => (g ^ x) ^ y = (g ^ y) ^ x.
 
 op [lossless full uniform] dssk: sskey distr.
 
 (** Instantiate the GapDH theory **)
 clone import St_CDH_abstract as StCDH with
-  type pkey       <= pdh,
-  type skey       <= sdh,
-  op   dkp        <= dkp,
-  op   shared_key <= shared_key
+  type pkey <= pdh,
+  type skey <= sdh,
+  op   g    <= g,
+  op   dsk  <= dsk,
+  op   (^)  <= (^)
 proof *.
-realize dkp_ll by exact: dkp_ll.
+realize dsk_ll by exact: dsk_ll.
 realize shared_keyC by exact: shared_keyC.
 
 (** Additional types for the signature scheme **)
@@ -67,9 +55,9 @@ proof *.
 (** Additional types for defining protocols,
     plus RO instantiation
 **)
-type client_state = { s_id: pkey;    (* The server's identity, as its public key *)
-                      x_pk: pdh;     (* The client's ephemeral public key *)
-                      x_sk: sdh   }. (* The client's ephemeral secret *)
+type client_state = { pk: pkey;     (* The server's identity, as its public key *)
+                      epk: pdh;     (* The client's ephemeral public key *)
+                      esk: sdh   }. (* The client's ephemeral secret *)
 
 clone import FullRO as H with
   type in_t    <= pdh * pdh * pdh,
@@ -105,34 +93,1259 @@ module SignedDH (S : SigScheme) (H : RO) : UATPaKE = {
     return kp;
   }
 
-  proc init(s_id) = {
-    var x_pk, x_sk;
+  proc init(pk) = {
+    var x_sk;
 
-    (x_pk, x_sk) <$ dkp;
-    return ({| s_id = s_id; x_pk = x_pk; x_sk = x_sk |}, x_pk);
+    x_sk <$ dsk;
+    return ({| pk = pk; epk = g ^ x_sk; esk = x_sk |}, g ^ x_sk);
   }
 
   proc resp(sk_s, x_pk) = {
-    var y_pk, y_sk, s, ss, ks;
+    var y_sk, s, ks;
 
-    (y_pk, y_sk) <$ dkp;
-    s <@ S.sign(sk_s, (x_pk, y_pk));
-    ss <- shared_key x_pk y_sk;
-    ks <@ H.get(ss, x_pk, y_pk);
-    return (ks, (y_pk, s));
+    y_sk <$ dsk;
+    s <@ S.sign(sk_s, (x_pk, g ^ y_sk));
+    ks <@ H.get(x_pk, g ^ y_sk, x_pk ^ y_sk);
+    return (ks, (g ^ y_sk, s));
   }
 
   proc recv(st, c) = {
-    var y_pk, s, b, ss, kc;
+    var y_pk, s, b, kc;
     var r <- None;
 
     (y_pk, s) <- c;
-    b <@ S.verify(s_id st, (x_pk st, y_pk), s);
+    b <@ S.verify(st.`pk, (st.`epk,  y_pk), s);
     if (b) {
-      ss <- shared_key y_pk (x_sk st);
-      kc <@ H.get(ss, x_pk st, y_pk);
+      kc <@ H.get(st.`epk, y_pk, y_pk ^ st.`esk);
       r <- Some kc;
     }
     return r;
   }
 }.
+
+module B1 (S : SigScheme) (A : Adv_UATPaKE_RO) (O : CMA_Oracles) = {
+  var b_ror : bool
+
+  var forgery : (int * (pdh * pdh) * sig) option
+
+  var n : int
+  var m : int
+  
+  var p_map : (int, int) fmap
+  var i_map : (int, pdh) fmap
+  var h_map : (pdh * pdh * pdh, sskey) fmap
+  var r_map : (int option * int, (pdh * sig) fset) fmap
+
+  var pk_map : (int, pkey) fmap
+  var c_map : (int, client_state) fmap
+  
+  var q : int fset
+  var ich : int fset
+  var rch : int fset
+  var xp : int fset
+  var cr : int fset
+  
+  module Oracles = {
+    proc gen(): pkey = {
+      var pk;
+
+      pk <@ O.gen();
+      if (has (fun i pk_i=> pk_i = pk /\ p_map.[i] = None) pk_map) {
+        pk <- witness;
+      } else {
+        m <- m + 1;
+        pk_map.[m] <- pk;
+      }
+      
+      return pk;
+    }
+
+    proc corrupt(j: int): skey option = {
+      var r <- None;
+
+      if (0 < j <= m) {
+        r <@ O.corrupt(j);
+        cr <- cr `|` fset1 j;
+      }
+      return r;
+    }
+
+    proc expose(i) = {
+      var r <- None;
+
+      if (0 < i <= n /\ i \notin ich) {
+        xp <- xp `|` fset1 i;
+        r <- c_map.[i];
+      }
+      return r;
+    }
+
+    proc init(pk: pkey): pdh = {
+      var st, jo, c, x;
+
+      n <- n + 1;
+      x <$ dsk;
+      c <- g ^ x;
+      st <- {| pk = pk; epk = c; esk = x; |};
+      c_map.[n] <- st;
+      jo <- find (fun _ pk_j=> pk_j = pk) pk_map;
+      if (jo is Some j) {
+        p_map.[n] <- j;
+        i_map.[n] <- c;
+      }
+      return c;
+    }
+
+    proc respond(j: int, c: pdh, ch: bool): (sskey * (pdh * sig)) option = {
+      var k, c', io, h, y, sig;
+      var r <- None;
+
+      if (0 < j <= m) {
+        y <$ dsk;
+        h <- g ^ y;
+        sig <@ O.sign(j, (c, h));
+        k <@ RO.get(c, h, c ^ y);
+        c' <- (h, oget sig);
+        io <- find (fun i j' => j' = j /\ i_map.[i] = Some c) p_map;
+        if (io is Some i) {
+          r_map.[Some j, i] <- (odflt fset0 r_map.[Some j, i]) `|` fset1 c';
+          if (ch /\ i \notin xp) {
+            if (b_ror) { k <$ dssk; }
+            ich <- ich `|` fset1 i;
+          }
+        }
+        r <- Some (k, c');
+      }
+      return r;
+    }
+
+    proc receive(i: int, c: pdh * sig, ch: bool): sskey option = {
+      var st_i, k, h, sig, b;
+      var ko <- None;
+
+      if (0 < i <= n /\ i \notin q) {
+        st_i <- oget c_map.[i];
+        q <- q `|` fset1 i;
+        
+        if (c \notin odflt fset0 r_map.[p_map.[i], i]) {
+          (h, sig) <- c;
+          b <@ S.verify(st_i.`pk, (st_i.`epk, h), sig);
+          if (b) {
+            k <@ RO.get(st_i.`epk, h, h ^ st_i.`esk);
+            ko <- Some k;
+          }
+          if (   ch
+              /\ i \notin xp
+              /\ p_map.[i] <> None /\ 0 < oget p_map.[i] <= m /\ oget p_map.[i] \notin cr
+              /\ ko <> None) {
+            if (forgery <> None) {
+              forgery <- Some (oget p_map.[i], (st_i.`epk, h), sig);
+            }
+            if (b_ror) { k <$ dssk; ko <- Some k; }
+            ich <- ich `|` fset1 i;
+          }
+        }
+      }
+      return ko;
+    }
+
+    proc h = RO.get
+  }
+
+  proc forge() = {
+    var b';
+
+    RO.init();
+
+    forgery <- None;
+
+    m <- 0;
+    n <- 0;
+
+    q <- fset0;
+    ich <- fset0;
+    rch <- fset0;
+    xp <- fset0;
+    cr <- fset0;
+
+    p_map <- empty;
+    i_map <- empty;
+    r_map <- empty;
+
+    pk_map <- empty;
+    c_map <- empty;
+
+    h_map <- empty;
+
+    b' <@ A(Oracles).distinguish();
+    return oget forgery;
+  }
+}.
+
+module B1_0 (S : SigScheme) (A : Adv_UATPaKE_RO) (O : CMA_Oracles) = {
+  proc forge() = {
+    var f;
+
+    B1.b_ror <- false;
+    f <@ B1(S, A, O).forge();
+    return f;
+  }
+}.
+
+module B1_1 (S : SigScheme) (A : Adv_UATPaKE_RO) (O : CMA_Oracles) = {
+  proc forge() = {
+    var f;
+
+    B1.b_ror <- true;
+    f <@ B1(S, A, O).forge();
+    return f;
+  }
+}.
+
+module B2 (S : SigScheme) (A : Adv_UATPaKE_RO) (O : St_CDH_Oracles) = {
+  include var Exp_b(SignedDH(S), RO, A) [-run]
+
+  var h_map : (pdh option * pdh * pdh, sskey) fmap
+
+  module Oracles = {
+    proc h'(x, y) = {
+      var k;
+
+      if ((None, x, y) \notin h_map) {
+        k <$ dssk;
+        h_map.[None, x, y] <- k;
+      }
+      return oget h_map.[None, x, y];
+    }
+
+    proc h(z, x, y) = {
+      var k, ko, b;
+
+      ko <- None;
+      if ((Some z, x, y) \notin h_map) {
+        b <@ O.ddh(x, y, z);
+        if (has (fun _ c=> c = x) i_map /\ b) {
+          k <@ h'(x, y);
+          ko <- Some k;
+        } else {
+          k <$ dssk;
+          h_map.[Some z, x, y] <- k;
+          ko <- Some k;
+        }
+      } else {
+        ko <- h_map.[Some z, x, y];
+      }
+      return oget ko;
+    }
+      
+    proc gen(): pkey = {
+      var pk, sk;
+
+      (pk, sk) <@ S.keygen();
+      if (has (fun i st=> st.`pk = pk /\ p_map.[i] = None) c_map) {
+        pk <- witness;
+      } else {
+        m <- m + 1;
+        pk_map.[m] <- pk;
+        sk_map.[m] <- sk;
+      }
+      
+      return pk;
+    }
+
+    proc corrupt(j: int): skey option = {
+      var r <- None;
+
+      if (0 < j <= m) {
+        r <- sk_map.[j];
+        cr <- cr `|` fset1 j;
+      }
+      return r;
+    }
+
+    proc expose(i) = {
+      var pk, x;
+      var r <- None;
+
+      if (0 < i <= n /\ i \notin ich) {
+        xp <- xp `|` fset1 i;
+        pk <- (oget c_map.[i]).`pk;
+        x <@ O.corrupt_1(i);
+        r <- Some {| pk = pk; epk = g ^ oget x; esk = oget x |};
+      }
+      return r;
+    }
+
+    proc init(pk: pkey): pdh = {
+      var st, jo, c;
+
+      n <- n + 1;
+      c <@ O.gen_1();
+      st <- {| pk = pk; epk = c; esk = witness; |};
+      c_map.[n] <- st;
+      jo <- find (fun _ pk_j=> pk_j = pk) pk_map;
+      if (jo is Some j) {
+        p_map.[n] <- j;
+        i_map.[n] <- c;
+      }
+      return c;
+    }
+
+    proc respond(j: int, c: pdh, ch: bool): (sskey * (pdh * sig)) option = {
+      var k, c', io, sk_j, h, y, sig;
+      var r <- None;
+
+      if (0 < j <= m) {
+        y <- witness; (* silence a warning: all paths that use y define it first *)
+        if (has (fun i j' => j' = j /\ i_map.[i] = Some c) p_map) {
+          h <@ O.gen_2();
+        } else {
+          y <$ dsk;
+          h <- g ^ y;
+        }
+        sk_j <- oget sk_map.[j];
+        sig <@ S.sign(sk_j, (c, h));
+        if (has (fun i j' => j' = j /\ i_map.[i] = Some c) p_map) {
+          k <@ h'(c, h);
+        } else {
+          k <@ RO.get(c, h, c ^ y);
+        }
+        c' <- (h, sig);
+        io <- find (fun i j' => j' = j /\ i_map.[i] = Some c) p_map;
+        if (io is Some i) {
+          (*** Instead of initialising all of r_map to output the
+          empty set, we read undefined entries as the empty set
+          here. ***)
+          r_map.[Some j, i] <- (odflt fset0 r_map.[Some j, i]) `|` fset1 c';
+          if (ch /\ i \notin xp) {
+            ich <- ich `|` fset1 i;
+          }
+        }
+        r <- Some (k, c');
+      }
+      return r;
+    }
+
+    proc receive(i: int, c: pdh * sig, ch: bool): sskey option = {
+      var st_i, k, h, sig, b;
+      var ko <- None;
+
+      if (0 < i <= n /\ i \notin q) {
+        st_i <- oget c_map.[i];
+        q <- q `|` fset1 i;
+        
+        if (c \notin odflt fset0 r_map.[p_map.[i], i]) {
+          (h, sig) <- c;
+          b <@ S.verify(st_i.`pk, (st_i.`epk, h), sig);
+          if (b) {
+            k <@ h'(st_i.`epk, h);
+            ko <- Some k;
+          }
+          if (   ch
+              /\ i \notin xp
+              /\ p_map.[i] <> None /\ 0 < oget p_map.[i] <= m /\ oget p_map.[i] \notin cr
+              /\ ko <> None) {
+            (* Spec says "Stop" *)
+            ich <- ich `|` fset1 i;
+          }
+        }
+      }
+      return ko;
+    }
+
+  }
+
+  proc solve() = {
+    var b';
+
+    RO.init();
+
+    b_ror <- witness;
+
+    m <- 0;
+    n <- 0;
+
+    q <- fset0;
+    ich <- fset0;
+    rch <- fset0;
+    xp <- fset0;
+    cr <- fset0;
+
+    p_map <- empty;
+    i_map <- empty;
+    r_map <- empty;
+
+    pk_map <- empty;
+    sk_map <- empty;
+    c_map <- empty;
+
+    h_map <- empty;
+
+    b' <@ A(Oracles).distinguish();
+  }
+}.
+
+section.
+declare module S <: SigScheme { -Exp_b, -SUFCMA, -RO, -B1, -B2 }.
+declare module A <: Adv_UATPaKE_RO { -Exp_b, -SUFCMA, -RO, -B1, -B2, -S }.
+
+local module Game0_b = {
+  include var Exp_b(SignedDH(S), RO, A) [-run]
+
+  module Oracles = {
+    proc gen(): pkey = {
+      var pk, sk;
+
+      m <- m + 1;
+      (pk, sk) <@ S.keygen();
+      pk_map.[m] <- pk;
+      sk_map.[m] <- sk;
+      return pk;
+    }
+
+    proc corrupt(j: int): skey option = {
+      var r <- None;
+
+      if (0 < j <= m) {
+        r <- sk_map.[j];
+        cr <- cr `|` fset1 j;
+      }
+      return r;
+    }
+
+    proc expose(i) = {
+      var r <- None;
+
+      if (0 < i <= n /\ i \notin ich) {
+        xp <- xp `|` fset1 i;
+        r <- c_map.[i];
+      }
+      return r;
+    }
+
+    proc init(pk: pkey): pdh = {
+      var st, jo, x, c;
+
+      n <- n + 1;
+      x <$ dsk;
+      c <- g ^ x;
+      st <- {| pk = pk; epk = c; esk = x |};
+      c_map.[n] <- st;
+      jo <- find (fun _ pk_j=> pk_j = pk) pk_map;
+      if (jo is Some j) {
+        p_map.[n] <- j;
+        i_map.[n] <- c;
+      }
+      return c;
+    }
+
+    proc respond(j: int, c: pdh, ch: bool): (sskey * (pdh * sig)) option = {
+      var k, c', io, sk_j, h, y, sig;
+      var r <- None;
+
+      if (0 < j <= m) {
+        sk_j <- oget sk_map.[j];
+        y <$ dsk;
+        h <- g ^ y;
+        sig <@ S.sign(sk_j, (c, h));
+        c' <- (h, sig);
+        k <@ RO.get(c, h, c ^ y);
+        io <- find (fun i _=> p_map.[i] = Some j /\ i_map.[i] = Some c) c_map;
+        if (io is Some i) {
+          (*** Instead of initialising all of r_map to output the
+          empty set, we read undefined entries as the empty set
+          here. ***)
+          r_map.[Some j, i] <- (odflt fset0 r_map.[Some j, i]) `|` fset1 c';
+          if (ch /\ i \notin xp) {
+            if (b_ror) { k <$ dssk; }
+            ich <- ich `|` fset1 i;
+          }
+        }
+        r <- Some (k, c');
+      }
+      return r;
+    }
+
+    proc receive(i: int, c: pdh * sig, ch: bool): sskey option = {
+      var st_i, k, h, sig, b;
+      var ko <- None;
+
+      if (0 < i <= n /\ i \notin q) {
+        st_i <- oget c_map.[i];
+        q <- q `|` fset1 i;
+        
+        if (c \notin odflt fset0 r_map.[p_map.[i], i]) {
+          (h, sig) <- c;
+          b <@ S.verify(st_i.`pk, (st_i.`epk, h), sig);
+          if (b) {
+            k <@ RO.get(st_i.`epk, h, h ^ st_i.`esk);
+            ko <- Some k;
+          }
+          if (   ch
+              /\ i \notin xp
+              /\ p_map.[i] <> None /\ 0 < oget p_map.[i] <= m /\ oget p_map.[i] \notin cr
+              /\ ko <> None) {
+            if (b_ror) { k <$ dssk; ko <- Some k; }
+            ich <- ich `|` fset1 i;
+          }
+        }
+      }
+      return ko;
+    }
+
+    proc h = RO.get
+  }
+
+  proc run(b) = {
+    var b';
+
+    RO.init();
+
+    b_ror <- b;
+
+    m <- 0;
+    n <- 0;
+
+    q <- fset0;
+    ich <- fset0;
+    rch <- fset0;
+    xp <- fset0;
+    cr <- fset0;
+
+    p_map <- empty;
+    i_map <- empty;
+    r_map <- empty;
+
+    pk_map <- empty;
+    sk_map <- empty;
+    c_map <- empty;
+
+    b' <@ A(Oracles).distinguish();
+    return b';
+  }
+}.
+
+local lemma Hop0 &m:
+  `|  Pr[Exp_b(SignedDH(S), RO, A).run(false) @ &m: res]
+    - Pr[Exp_b(SignedDH(S), RO, A).run(true ) @ &m: res] |
+  = `|  Pr[Game0_b.run(false) @ &m: res]
+      - Pr[Game0_b.run(true ) @ &m: res] |.
+proof.
+have ^ + -> - -> //:
+  forall b, Pr[Exp_b(SignedDH(S), RO, A).run(b) @ &m: res]
+          = Pr[Game0_b.run(b) @ &m: res].
+move=> b; byequiv (: ={glob A, glob S, arg} ==> ={res})=> //.
+proc.
+(* The calls are equivalent due to equality on a bunch of variables *)
+call (: ={glob Exp_b(SignedDH(S), RO)}); last first.
+(* The invariant holds initially and allows us to conclude *)
++ by inline *; auto.
+(* The invariant is preserved by all oracles *)
++ by proc; inline *; auto; call (: true); auto.
++ by proc; inline *; auto.
++ by proc; inline *; auto.
++ by proc; inline *; sim; auto.
++ proc; inline *; sp; if; auto.
+  sim; auto.
+  by call (: true); auto.
++ proc; sp; if; auto; sp; if; auto.
+  inline {1} 1.
+  by sim; auto.
++ conseq (: _ ==> ={glob RO, res})=> //.
+  by sim.
+qed.
+
+local module Game1_b = {
+  include var Exp_b(SignedDH(S), RO, A) [-run]
+
+  var bad_1: bool
+  var bad_2: bool
+
+  module Oracles = {
+    include Game0_b.Oracles [-gen]
+
+    proc gen(): pkey = {
+      var pk, sk;
+  
+      (pk, sk) <@ S.keygen();
+      if (has (fun i st=> st.`pk = pk /\ p_map.[i] = None) c_map) {
+        bad_1 <- true;
+        (* Pen and paper says "Stop" *)
+        (* Here, we don't stop; we just don't actually register the key and move on *)
+        (* The only thing we care about is the rest of the proof,
+           where we want to rely on the fact that each client instance
+           has at most one intended honest partner
+        *)
+        pk <- witness;
+      } else {
+        m <- m + 1;
+        pk_map.[m] <- pk;
+        sk_map.[m] <- sk;
+      }
+      
+      return pk;
+    }
+  }
+
+  proc run(b) = {
+    var b';
+
+    RO.init();
+
+    b_ror <- b;
+
+    m <- 0;
+    n <- 0;
+
+    q <- fset0;
+    ich <- fset0;
+    rch <- fset0;
+    xp <- fset0;
+    cr <- fset0;
+
+    p_map <- empty;
+    i_map <- empty;
+    r_map <- empty;
+
+    pk_map <- empty;
+    sk_map <- empty;
+    c_map <- empty;
+
+    bad_1 <- false;
+    bad_2 <- false;
+
+    b' <@ A(Oracles).distinguish();
+    return b';
+  }
+}.
+
+local module Game2_b = {
+  include var Exp_b(SignedDH(S), RO, A) [-run]
+  include var Game1_b [-run]
+
+  module Oracles = {
+    proc gen(): pkey = {
+      var pk, sk;
+
+      (pk, sk) <@ S.keygen();
+      if (has (fun i st=> st.`pk = pk /\ p_map.[i] = None) c_map) {
+        bad_1 <- true;
+        (* Here, we don't stop; we just don't actually register the key and move on *)
+        pk <- witness;
+      } else {
+        m <- m + 1;
+        pk_map.[m] <- pk;
+        sk_map.[m] <- sk;
+      }
+      
+      return pk;
+    }
+
+    proc corrupt(j: int): skey option = {
+      var r <- None;
+
+      if (0 < j <= m) {
+        r <- sk_map.[j];
+        cr <- cr `|` fset1 j;
+      }
+      return r;
+    }
+
+    proc expose(i) = {
+      var r <- None;
+
+      if (0 < i <= n /\ i \notin ich) {
+        xp <- xp `|` fset1 i;
+        r <- c_map.[i];
+      }
+      return r;
+    }
+
+    proc init(pk: pkey): pdh = {
+      var st, jo, c, x;
+
+      n <- n + 1;
+      x <$ dsk;
+      c <- g ^ x;
+      st <- {| pk = pk; epk = c; esk = x |};
+      c_map.[n] <- st;
+      jo <- find (fun _ pk_j=> pk_j = pk) pk_map;
+      if (jo is Some j) {
+        p_map.[n] <- j;
+        i_map.[n] <- c;
+      }
+      return c;
+    }
+
+    proc respond(j: int, c: pdh, ch: bool): (sskey * (pdh * sig)) option = {
+      var k, c', io, sk_j, h, y, sig;
+      var r <- None;
+
+      if (0 < j <= m) {
+        sk_j <- oget sk_map.[j];
+        y <$ dsk;
+        h <- g ^ y;
+        sig <@ S.sign(sk_j, (c, h));
+        c' <- (h, sig);
+        k <@ RO.get(c, h, c ^ y);
+        io <- find (fun i _=> p_map.[i] = Some j /\ i_map.[i] = Some c) c_map;
+        if (io is Some i) {
+          (*** Instead of initialising all of r_map to output the
+          empty set, we read undefined entries as the empty set
+          here. ***)
+          r_map.[Some j, i] <- (odflt fset0 r_map.[Some j, i]) `|` fset1 c';
+          if (ch /\ i \notin xp) {
+            if (b_ror) { k <$ dssk; }
+            ich <- ich `|` fset1 i;
+          }
+        }
+        r <- Some (k, c');
+      }
+      return r;
+    }
+
+    proc receive(i: int, c: pdh * sig, ch: bool): sskey option = {
+      var st_i, k, h, sig, b;
+      var ko <- None;
+
+      if (0 < i <= n /\ i \notin q) {
+        st_i <- oget c_map.[i];
+        q <- q `|` fset1 i;
+        
+        if (c \notin odflt fset0 r_map.[p_map.[i], i]) {
+          (h, sig) <- c;
+          b <@ S.verify(st_i.`pk, (st_i.`epk, h), sig);
+          if (b) {
+            k <@ RO.get(st_i.`epk, h, h ^ st_i.`esk);
+            ko <- Some k;
+          }
+          if (   ch
+              /\ i \notin xp
+              /\ p_map.[i] <> None /\ 0 < oget p_map.[i] <= m /\ oget p_map.[i] \notin cr
+              /\ ko <> None) {
+            bad_2 <- true;
+            ko <- None;
+            ich <- ich `|` fset1 i;
+          }
+        }
+      }
+      return ko;
+    }
+
+    proc h = RO.get
+  }
+
+  proc run(b) = {
+    var b';
+
+    RO.init();
+
+    b_ror <- b;
+
+    m <- 0;
+    n <- 0;
+
+    q <- fset0;
+    ich <- fset0;
+    rch <- fset0;
+    xp <- fset0;
+    cr <- fset0;
+
+    p_map <- empty;
+    i_map <- empty;
+    r_map <- empty;
+
+    pk_map <- empty;
+    sk_map <- empty;
+    c_map <- empty;
+
+    bad_1 <- false;
+    bad_2 <- false;
+
+    b' <@ A(Oracles).distinguish();
+    return b';
+  }
+}.
+
+(** We now successively state and prove claims about consecutive games
+    in the sequence. We sometimes introduce intermediate modules as
+    proof artefacts to enable formal reasoning.
+**)
+
+(** Hop 1: Game 0 and Game 1 are equivalent (regardless of the value
+    of the challenge bit) unless (and until) the gen oracle outputs a
+    public key that was already used by the adversary.
+
+    This happens with a probability bounded by the guessing entropy of
+    the distribution induced on public keys by key generation.
+**)
+local lemma Hop1 (b : bool) &m:
+  `|Pr[Game0_b.run(b) @ &m: res] - Pr[Game1_b.run(b) @ &m: res]|
+  <= Pr[Game1_b.run(b) @ &m: Game1_b.bad_1].
+(* This aborts the proof - we simply use the statement as a section heading. *)
+abort.
+
+(* In order to get the absolute values in, we need to make sure that
+   we can express the bad event on the left of the hop. While we do
+   this, we also set things up nicely to avoid having to reason about
+   equivalence up to bad in manual mode.
+*)
+local module Game05_b = {
+  include var Exp_b(SignedDH(S), RO, A) [-run]
+  include var Game1_b [-run]
+
+  module Oracles = {
+    (* The oracles are unchanged from Game1, except for gen *)
+    include Game1_b.Oracles [-gen]
+
+    proc gen(): pkey = {
+      var pk, sk;
+  
+      (pk, sk) <@ S.keygen();
+      if (has (fun i st=> st.`pk = pk /\ p_map.[i] = None) c_map) {
+        bad_1 <- true;
+        m <- m + 1;
+        pk_map.[m] <- pk;
+        sk_map.[m] <- sk;
+      } else {
+        m <- m + 1;
+        pk_map.[m] <- pk;
+        sk_map.[m] <- sk;
+      }
+      
+      return pk;
+    }
+  }
+
+  proc run(b) = {
+    var b';
+
+    RO.init();
+
+    b_ror <- b;
+
+    m <- 0;
+    n <- 0;
+
+    q <- fset0;
+    ich <- fset0;
+    rch <- fset0;
+    xp <- fset0;
+    cr <- fset0;
+
+    p_map <- empty;
+    i_map <- empty;
+    r_map <- empty;
+
+    pk_map <- empty;
+    sk_map <- empty;
+    c_map <- empty;
+
+    bad_1 <- false;
+    bad_2 <- false;
+
+    b' <@ A(Oracles).distinguish();
+    return b';
+  }
+}.
+
+(** Despite setting things up, the syntactic 'equivalent up to' tactic
+    is failing here for some reason. So we must do it by hand, which
+    requires us assuming that the adversary and the signature scheme
+    terminate.
+
+    This can pop off once the bugs in `byupto` are fixed.
+**)
+(* For all oracles that terminate, the adversary terminates *)
+declare axiom A_ll (O <: UATPaKE_RO_Oracles {-A}):
+     islossless O.gen
+  => islossless O.corrupt
+  => islossless O.expose
+  => islossless O.init
+  => islossless O.respond
+  => islossless O.receive
+  => islossless O.h
+  => islossless A(O).distinguish.
+
+declare axiom S_keygen_ll: islossless S.keygen.
+declare axiom S_sign_ll: islossless S.sign.
+declare axiom S_verify_ll: islossless S.verify.
+
+local lemma Hop1 (b : bool) &m:
+  `|Pr[Game0_b.run(b) @ &m: res] - Pr[Game1_b.run(b) @ &m: res]|
+  <= Pr[Game1_b.run(b) @ &m: Game1_b.bad_1].
+proof.
+(* We need to make the bad event appear in the left game for the
+   absolute value to work out; this is just a pure equivalence
+   with a bit of a twist, since we modify *one* of the oracles
+   to branch on the failure event and set bad, but without changing
+   its obserable behaviour. The proof quickly focuses on this. *)
+have ->: Pr[Game0_b.run(b) @ &m: res] = Pr[Game05_b.run(b) @ &m: res].
++ byequiv (: ={glob A, glob S, b} ==> ={res})=> //; proc.
+  call (: ={glob Exp_b, glob S, glob RO}); [2..7:by sim|8:by inline; auto].
+  by proc; auto; call (: true); auto=> />.
+(* Now, in theory, this could be done by the syntactic check: those
+   two games are syntactically equal except in branches that set bad
+   to true. However, this is borked right now, so we breathe in manual
+   mode, and we prove _semantically_ that:
+   1. Some invariant holds until bad happens, and implies the desired
+   equality of events in final memories;
+   2. Bad happens on both sides at the same time.
+*)
+byequiv: Game1_b.bad_1=> [||/#] //.
+proc.
+(* And now we lift the reasoning up to bad to the oracles the
+   adversary has access to. Because we're in manual mode, and the
+   semantics of `equiv` imply equitermination, we *must* also show that
+   everything terminates once bad has occurred (we can no longer rely on
+   the relational reasoning to guarantee thise once the programs are out
+   of sync). In addition, and perhaps obviously, we must prove that
+   the bad even can never unhappen once it has happened.  Keep in mind
+   that it is simply a property of the state (here, the value of a
+   boolean variable), and that the state can be modified
+   programmatically. It isn't some external, untouchable truth. *)
+call (: Game1_b.bad_1 (* the bad event *)
+      , ={glob Exp_b, glob S, glob RO, Game1_b.bad_1, Game1_b.bad_2} (* the invariant that holds until bad happens *)
+      , ={Game1_b.bad_1}). (* the invariant that holds after bad happens *)
+(* Goal 1: the adversary terminates if its oracles terminate. See above. *)
++ exact: A_ll.
+(* Goal i.0: if bad does not hold, and the non-bad invariant holds
+   initially, then executing the oracles leads us to memories that are
+   such that the correct invariant holds (depending on whether bad
+   happened during the oracles' execution *)
++ by proc; auto; call (: true); auto.
+(* Goal i.1: the left-hand side oracle terminates and preserves bad *)
++ move=> &2 bad; proc; auto=> />.
+  by call S_keygen_ll; auto=> />; rewrite bad.
+(* Goal i.2: the right-hand side oracle terminates and preserves bad *)
++ move=> &1; proc; auto.
+  by call S_keygen_ll; auto=> />.
+(* Do those three again for all oracles *)
++ conseq (: ={glob Exp_b, glob S, glob RO, Game1_b.bad_1, Game1_b.bad_2, res})=> //.
+  by sim.
++ by move=> &2 bad; proc; auto.
++ by move=> &1; proc; auto.
+(* And again *)
++ conseq (: ={glob Exp_b, glob S, glob RO, Game1_b.bad_1, Game1_b.bad_2, res})=> //.
+  by sim.
++ by move=> &2 bad; proc; auto.
++ by move=> &1; proc; auto.
+(* And again *)
++ conseq (: ={glob Exp_b, glob S, glob RO, Game1_b.bad_1, Game1_b.bad_2, res})=> //.
+  by sim.
++ move=> &2 bad; proc; auto=> /> &0.
+  by rewrite dsk_ll /= /#.
++ move=> &1; proc; auto=> /> &0.
+  by rewrite dsk_ll /= /#.
+(* And again *)
++ conseq (: ={glob Exp_b, glob S, glob RO, Game1_b.bad_1, Game1_b.bad_2, res})=> //.
+  by sim.
++ move=> &2 bad; conseq (: true); proc; islossless.
+  + by match; islossless.
+  + exact: S_sign_ll.
++ move=> &1; conseq (: true); proc; islossless.
+  + by match; islossless.
+  + exact: S_sign_ll.
+(* And again *)
++ conseq (: ={glob Exp_b, glob S, glob RO, Game1_b.bad_1, Game1_b.bad_2, res})=> //.
+  by sim.
++ move=> &2 bad; conseq (: true); proc; islossless.
+  exact: S_verify_ll.
++ move=> &1; conseq (: true); proc; islossless.
+  exact: S_verify_ll.
+(* And again *)
++ conseq (: ={glob Exp_b, glob S, glob RO, Game1_b.bad_1, Game1_b.bad_2, res})=> //.
+  by sim.
++ by move=> &2 bad; conseq (: true); proc; islossless.
++ by move=> &1; conseq (: true); proc; islossless.
+(* Finally, show that the invariant implies what we wanted (and that
+   the program's preamble establishes the invariant) *)
+by inline; auto=> /> /#.
+qed.
+
+(** Hop 2: Game 1 and Game 2 are equivalent unless (and until) the
+    adversary successfully triggers bad_2 in Game 2.
+**)
+local lemma Hop2 b &m:
+  `|Pr[Game1_b.run(b) @ &m: res] - Pr[Game2_b.run(b) @ &m: res]|
+  <= Pr[Game2_b.run(b) @ &m: Game1_b.bad_2].
+admitted.
+
+(** Reduction for Hop 2: If bad_2 happens, then we can extract a
+    forgery, regardless of the challenge bit.
+**)
+local lemma Reduction1 b &m:
+     B1.b_ror{m} = b
+  => Pr[Game2_b.run(b) @ &m: Game1_b.bad_2]
+     <= Pr[SUFCMA(S, B1(S, A)).run() @ &m: res].
+abort.
+
+(* We'd need to prove the same thing twice (once for each b) if we
+   prove it directly on probabilities. But we can be a bit more clever
+   by going one level down.
+*)
+local equiv Reduction1_equiv:
+  Game2_b.run ~ SUFCMA(S, B1(S, A)).run:
+       ={glob A, glob S, glob RO}
+    /\ b{1} = B1.b_ror{2}
+    ==> Game1_b.bad_2{1} => res{2}.
+(** HERE BE DRAGONS: we cannot immediately conclude that running
+    verification after the adversary returns (on the right) will
+    always give the same result as running it before the adversary's
+    run concludes (on the left). Here, we might just need to actually
+    halt and prevent the adversary to trigger more signing on the
+    left. (Or to restrict the class of signing algorithms the result
+    applies to, to a very reasonable class of algorithms where "if
+    verification succeeds once, then it succeeds every time on the
+    same input". This is slightly less reasonable if we want to allow
+    for stateful signature schemes...
+**)
+admitted.
+
+local lemma Reduction1_0 &m:
+  Pr[Game2_b.run(false) @ &m: Game1_b.bad_2]
+  <= Pr[SUFCMA(S, B1_0(S, A)).run() @ &m: res].
+proof.
+byequiv (: ={glob A, glob S, glob RO} /\ !b{1} ==> Game1_b.bad_2{1} => res{2})=> //.
+proc *.
+transitivity {2}
+  { B1.b_ror <- false;
+    r <@ SUFCMA(S, B1(S, A)).run(); }
+  (={glob A, glob S, glob RO} /\ !b{1} ==> Game1_b.bad_2{1} => r{2})
+  (={glob A, glob S, glob RO} ==> ={r})=> [/#|/>||].
++ by call Reduction1_equiv; auto=> />.
++ inline *; swap {2} 7 -6.
+  sim; wp=> />.
+  by sim: (={B1.forgery, b, SUFCMA.q, SUFCMA.cr, SUFCMA.pk_map, SUFCMA.n, glob S})=> />.
+qed.
+
+local lemma Reduction1_1 &m:
+  Pr[Game2_b.run(true) @ &m: Game1_b.bad_2]
+  <= Pr[SUFCMA(S, B1_1(S, A)).run() @ &m: res].
+proof.
+byequiv (: ={glob A, glob S, glob RO} /\ b{1} ==> Game1_b.bad_2{1} => res{2})=> //.
+proc *.
+transitivity {2}
+  { B1.b_ror <- true;
+    r <@ SUFCMA(S, B1(S, A)).run(); }
+  (={glob A, glob S, glob RO} /\ b{1} ==> Game1_b.bad_2{1} => r{2})
+  (={glob A, glob S, glob RO} ==> ={r})=> [/#|/>||].
++ by call Reduction1_equiv; auto=> />.
++ inline *; swap {2} 7 -6.
+  sim; wp=> />.
+  by sim: (={B1.forgery, b, SUFCMA.q, SUFCMA.cr, SUFCMA.pk_map, SUFCMA.n, glob S})=> />.
+qed.
+
+local module Game3_b = {
+  include var Exp_b(SignedDH(S), RO, A) [-run]
+  include var Game1_b [-run]
+
+  var h_map : (pdh option * pdh * pdh, sskey) fmap
+
+  module Oracles = {
+    proc h'(x, y) = {
+      var k;
+
+      if ((None, x, y) \notin h_map) {
+        k <$ dssk;
+        h_map.[None, x, y] <- k;
+      }
+      return oget h_map.[None, x, y];
+    }
+
+    proc h(z, x, y) = {
+      var io, st_i, k, ko;
+
+      ko <- None;
+      if ((Some z, x, y) \notin h_map) {
+        io <- find (fun _ c=> c = x) i_map;
+        if (io is Some i) {
+          st_i <- oget c_map.[i];
+          if (z = y ^ st_i.`esk) {
+            k <@ h'(x, y);
+            ko <- Some k;
+          }
+        }
+        if (ko is None) {
+          k <$ dssk;
+          h_map.[Some z, x, y] <- k;
+          ko <- Some k;
+        }
+      } else {
+        ko <- h_map.[Some z, x, y];
+      }
+      return oget ko;
+    }
+      
+    proc gen(): pkey = {
+      var pk, sk;
+
+      (pk, sk) <@ S.keygen();
+      if (has (fun i st=> st.`pk = pk /\ p_map.[i] = None) c_map) {
+        bad_1 <- true;
+        (* Here, we don't stop; we just don't actually register the key and move on *)
+        pk <- witness;
+      } else {
+        m <- m + 1;
+        pk_map.[m] <- pk;
+        sk_map.[m] <- sk;
+      }
+      
+      return pk;
+    }
+
+    proc corrupt(j: int): skey option = {
+      var r <- None;
+
+      if (0 < j <= m) {
+        r <- sk_map.[j];
+        cr <- cr `|` fset1 j;
+      }
+      return r;
+    }
+
+    proc expose(i) = {
+      var r <- None;
+
+      if (0 < i <= n /\ i \notin ich) {
+        xp <- xp `|` fset1 i;
+        r <- c_map.[i];
+      }
+      return r;
+    }
+
+    proc init(pk: pkey): pdh = {
+      var st, jo, c, x;
+
+      n <- n + 1;
+      x <$ dsk;
+      c <- g ^ x;
+      st <- {| pk = pk; epk = c; esk = x |};
+      c_map.[n] <- st;
+      jo <- find (fun _ pk_j=> pk_j = pk) pk_map;
+      if (jo is Some j) {
+        p_map.[n] <- j;
+        i_map.[n] <- c;
+      }
+      return c;
+    }
+
+    proc respond(j: int, c: pdh, ch: bool): (sskey * (pdh * sig)) option = {
+      var k, c', io, sk_j, h, y, sig;
+      var r <- None;
+
+      if (0 < j <= m) {
+        sk_j <- oget sk_map.[j];
+        y <$ dsk;
+        h <- g ^ y;
+        sig <@ S.sign(sk_j, (c, h));
+        c' <- (h, sig);
+        if (has (fun i c' => c' = c) i_map) {
+          k <@ h'(c, h);
+        } else {
+          k <@ RO.get(c, h, c ^ y);
+        }
+        io <- find (fun i _=> p_map.[i] = Some j /\ i_map.[i] = Some c) c_map;
+        if (io is Some i) {
+          (*** Instead of initialising all of r_map to output the
+          empty set, we read undefined entries as the empty set
+          here. ***)
+          r_map.[Some j, i] <- (odflt fset0 r_map.[Some j, i]) `|` fset1 c';
+          if (ch /\ i \notin xp) {
+            if (b_ror) { k <$ dssk; }
+            ich <- ich `|` fset1 i;
+          }
+        }
+        r <- Some (k, c');
+      }
+      return r;
+    }
+
+    proc receive(i: int, c: pdh * sig, ch: bool): sskey option = {
+      var st_i, k, h, sig, b;
+      var ko <- None;
+
+      if (0 < i <= n /\ i \notin q) {
+        st_i <- oget c_map.[i];
+        q <- q `|` fset1 i;
+        
+        if (c \notin odflt fset0 r_map.[p_map.[i], i]) {
+          (h, sig) <- c;
+          b <@ S.verify(st_i.`pk, (st_i.`epk, h), sig);
+          if (b) {
+            k <@ h'(st_i.`epk, h);
+            ko <- Some k;
+          }
+          if (   ch
+              /\ i \notin xp
+              /\ p_map.[i] <> None /\ 0 < oget p_map.[i] <= m /\ oget p_map.[i] \notin cr
+              /\ ko <> None) {
+            bad_2 <- true;
+            if (b_ror) { k <$ dssk; ko <- Some k; }
+            ich <- ich `|` fset1 i;
+          }
+        }
+      }
+      return ko;
+    }
+
+  }
+
+  proc run(b) = {
+    var b';
+
+    RO.init();
+
+    b_ror <- b;
+
+    m <- 0;
+    n <- 0;
+
+    q <- fset0;
+    ich <- fset0;
+    rch <- fset0;
+    xp <- fset0;
+    cr <- fset0;
+
+    p_map <- empty;
+    i_map <- empty;
+    r_map <- empty;
+
+    pk_map <- empty;
+    sk_map <- empty;
+    c_map <- empty;
+
+    bad_1 <- false;
+    bad_2 <- false;
+
+    h_map <- empty;
+
+    b' <@ A(Oracles).distinguish();
+    return b';
+  }
+}.
+
+op p: real.
+local lemma Hop3 b &m:
+  `|Pr[Game2_b.run(b) @ &m: res] - Pr[Game3_b.run(b) @ &m: res]|
+  <= p.
+admitted.
+
+local lemma Reduction &m:
+  `|Pr[Game3_b.run(false) @ &m: res] - Pr[Game3_b.run(true) @ &m: res]|
+  <= Pr[St_CDH(B2(S,A)).run() @ &m: res].
+proof. admitted.
+
+local lemma Security_of_SignedDH &m:
+  `|  Pr[Exp_b(SignedDH(S), RO, A).run(false) @ &m : res]
+    - Pr[Exp_b(SignedDH(S), RO, A).run(true) @ &m : res]|
+  <=   Pr[Game1_b.run(true) @ &m: Game1_b.bad_1]
+     + Pr[Game1_b.run(false) @ &m: Game1_b.bad_1]
+     + Pr[SUFCMA(S, B1_0(S, A)).run() @ &m: res]
+     + Pr[SUFCMA(S, B1_1(S, A)).run() @ &m: res]
+     + 2%r * p
+     + Pr[St_CDH(B2(S,A)).run() @ &m: res].
+proof.
+smt(Hop0 Hop1 Hop2 Reduction1_0 Reduction1_1 Hop3 Reduction).
+qed.
+end section.
